working prototype message inv generator

messageInvariantPrototypes/ringLeaderElection/automate/parser.py
@@ -1,46 +1,20 @@
 import collections
 import re
+import sys
+import msgInv
 
 SEND_PREDICATE_KEYWORD = "sendPredicate"
 
-class Module:
-    def __init__(self, raw):
-        self.raw_string = raw
-        self.name = "mod_name"
-        self.send_predicates = []
-    
-    def add_predicate(self, new_pred):
-        self.send_predicates.append(new_pred)
-
-    def __str__(self):
-        res = []
-        res.append("module " + self.name + ":")
-        if len(self.send_predicates) == 0:
-            res.append("   " + "no send predicates")
-        
-        for sp in self.send_predicates:
-            res.append("   " + sp.__str__())
-        res.append("")
-        return "\n".join(res)
-
-class SendPredicate:
-    def __init__(self, name = "sp_name", hosts_field = "hosts"):
-        self.name = name
-        self.hosts_field = hosts_field
-
-    def __str__(self):
-        return self.name + ": " + self.host_field
-
 """Returns Module list"""
-def parse(hf):
+def parse(hosts_file):
     def skip_line(line):
         return line.strip() == "" or "include" in line
     
     res = []
     curr_module = []
     open_braces = 0
-    for line in hf:
-        if skip_line(line) and open_braces == 0:
+    for line in hosts_file:
+        if open_braces == 0 and skip_line(line):
             continue
         all_counts = collections.Counter(line)
         open_braces += all_counts["{"]
@@ -48,30 +22,42 @@ def parse(hf):
         curr_module.append(line)
         if open_braces == 0:
             res.append(parse_module(curr_module))
-            # reset
+             # Reset after parsing each module
             curr_module = []
-            open_braces = 0
     return res
 
 """Returns Module"""
 def parse_module(module_lines):
-    res = Module("".join(module_lines))
+    module = msgInv.Module("".join(module_lines))
 
     # Scan for Send Predicates
     lines_iter = iter(module_lines)
     line = next(lines_iter)
-    res.name = re.split(' |\{', line)[1]
-    try:
-        while True:
+    module.name = re.split(' |\{', line)[1]
+    while True:
+        try:
             line = next(lines_iter)
             # Found a Send Predicate
             if SEND_PREDICATE_KEYWORD in line:
-                sp = SendPredicate()
-                sp.host_field = re.sub(" |[^0-9a-zA-Z\s]+", "", line.split(":")[1]).strip()
+                predicate = msgInv.SendPredicate(module.name)
+                attributes_string = line.split(":")[1]
+                predicate.host_field = attributes_string.split(",")[0].strip()
+                predicate.msg_cons = attributes_string.split(",")[1].strip()
                 while "ghost predicate" not in line:
                     line = next(lines_iter)
-                sp.name = re.split(' |\(', line)[4].strip()
-                res.add_predicate(sp)
-    except StopIteration:
-        pass
-    return res
+                predicate.name = re.split(" |\(", line)[4].strip()
+                module.add_predicate(predicate)
+        except StopIteration:
+            break
+    return module
+
+def main():
+    args = sys.argv[1:]
+    host_file = args[0]
+    with open(host_file, "r+") as host_file:
+        modules = parse(host_file)
+        msg_inv_file = msgInv.MessageInvariantsFile(modules)
+        print(msg_inv_file.to_dafny_string())
+    
+if __name__ == "__main__":
+    main()
